\begin{enumerate}[label=(\alph*)]
\item Let $S$ be the sum of the ranks of the dishes we eat during both phases.
$S = (m-k+1)X + \sum_{j=1}^{k-1}R_{j}$, where $R_{j}$ is the rank of dish $j$,
excluding the highest ranked dish, from the exploration phase. Since $\text{E}
(R_{j}) = \frac{(X-1)X}{2} \times \frac{\binom{X-2}{k-2}}{(k-1)\binom{X-1}{k-1}}
=
\frac{(X-1)X}{2} \times \frac{1}{X-1} = \frac{X}{2}$, $
\text{E}(S) = (m-k+1)\text{E}(X) + (k-1)\frac{\text{E}(X)}{2} = (m-k)\text{E}
(X) + (k+1)\frac{\text{E}(X)}{2}.$

\item $P(X = x) = \frac{\binom{x-1}{k-1}}{\binom{n}{k}}.$

\item 
\begin{flalign}
\text{E}(X) & = \frac{1}{\binom{n}{k}}\sum_{i=k}^{n}i\binom{i-1}{k-1} \nonumber \\
& = \frac{1}{\binom{n}{k}}\sum_{i=k}^{n}k\binom{i}{k} \nonumber \\
& = \frac{k}{\binom{n}{k}}\sum_
{i=k}^{n}\binom{i}{k} \nonumber \\
& = \frac{k}{\binom{n}{k}}\binom{n+1}{k+1} \nonumber \\
& = \frac{k(n+1)}{k+1} \nonumber
\end{flalign}

\item Plugging $\frac{k(n+1)}{k+1}$ into the result of part $b$ and derivating $
(m-k)\frac{k(n+1)}{k+1} + k\frac{n+1}{2}$ with respect to $k$
provides an extremum of $k = \sqrt{2(m+1)} - 1$.

\end{enumerate}