\begin{enumerate}[label=(\alph*)]
\item 
\begin{align*}
\text{E}(Xg(X)) &= \sum_{x=0}^{\infty}xg(x)\frac{\text{e}^{-\lambda}
(\lambda)^{x}}{x!} \\
&= \sum_{x=1}^{\infty}xg(x)\frac{\text{e}^{-\lambda}
(\lambda)^{x}}{x!} \\
&= \lambda\sum_{x=1}^{\infty}g(x)\frac{\text{e}^{-\lambda}
(\lambda)^{x-1}}{(x-1)!} \\
&= \lambda\sum_{x=0}^{\infty}g(x+1)\frac{\text{e}^{-\lambda}
(\lambda)^{x}}{(x)!} = \lambda\text{E}(g(X+1))
\end{align*}

\item 
\begin{align*}
\text{E}(X^{3}) &= \text{E}(XX^{2}) \\
&= \lambda\text{E}((X+1)^{2}) \\
&= \lambda(\text{E}(X^{2}) + \text{E}(2X) + 1) \\
&= \lambda(\lambda\text{E}(X+1) +
2\lambda + 1) = \lambda(\lambda(\lambda + 1) + 2\lambda + 1) \\
&= \lambda(\lambda^{2} + 3\lambda + 1)
\end{align*}
\end{enumerate}
