\begin{enumerate}[label=(\alph*)]
\item By the story of the problem, $X \sim \text{NHGeom}(n, N-n, m)$. Then, $Y =
X + m$.

\item According to part $a$, $\text{E}(Y) = \text{E}(X) + m = \frac{m(N-n)}
{n+1} + m$. The implied indicator variables are the same as in the proof of the
expectation of Negative Hypergeometric random variables.

\item The problem can be modeled with a Hypergeometric random variable $Z
\sim \text{HGeom}(n, N-n, \text{E}(Y))$. Then, $\text{E}(Z) = \text{E}
(Y)\frac{n}{N} = (\frac{m(N-n)}{n+1} + m)\frac{n}{N} = m \times \frac{N+1}
{n+1}\times
\frac{n}{N}$. Since $\frac{N+1}{n+1} \times \frac{n}{N} < 1 \implies (n+1)N(n-N)
< 0 \implies \frac{N-n}{(n+1)N} > 0 \implies n < N$ for positive $n$ and $N$, $
\text{E}(Z) < m$.
\end{enumerate}